backend/Linearizeproof.v
@@ -15,7 +15,7 @@
 Require Import FSets.
 Require Import Coqlib Maps Ordered Errors Lattice Kildall Integers.
 Require Import AST Linking.
-Require Import Values Memory Events Globalenvs Smallstep ExposedSmallstep.
+Require Import Values Memory Events Globalenvs Smallstep ExposedSimulations.
 Require Import Op Locations LTL Linear.
 Require Import Linearize.
 
@@ -735,6 +735,19 @@ Proof.
   constructor. constructor. auto.
 Qed.
 
+Lemma transf_initial_states':
+  forall s1 : LTL.state,
+  Smallstep.initial_state (LTL.semantics prog) s1 ->
+  exists s2 : state,
+    Smallstep.initial_state (semantics tprog) s2 /\ match_states s1 s2.
+Proof.
+  eapply (@init_states_from_entry (LTL.semantics prog) (semantics tprog));
+    try apply transf_entry_points.
+  - apply (Genv.init_mem_match TRANSF); eauto.
+  - simpl. destruct TRANSF as (P & Q & R). auto.
+    rewrite symbols_preserved, Q; auto.
+Qed.
+
 Lemma transf_final_states:
   forall st1 st2 r,
   match_states st1 st2 -> LTL.final_state st1 r -> Linear.final_state st2 r.
@@ -748,7 +761,7 @@ Proof.
   eapply forward_simulation_star.
   apply senv_preserved.
   eexact transf_entry_points.
-  eexact transf_initial_states.
+  eexact transf_initial_states'.
   eexact transf_final_states.
   eexact transf_step_correct.
 Qed.
@@ -758,9 +771,10 @@ Qed.
                   _ (ltof _ measure)
                   ( fun idx s1 s2 => idx = s1 /\ match_states s1 s2).
 Proof.
-  eapply forward_simulation_star'.
+  eapply fsim_properties_star.
   apply senv_preserved.
-  eexact transf_initial_states.
+  eexact transf_entry_points.
+  eexact transf_initial_states'.
   eexact transf_final_states.
   eexact transf_step_correct.
 Qed.
